examples/conflicts_modular.v
@@ -1,33 +1,245 @@
 (*! Understanding conflicts and forwarding, with modules !*)
-Require Import Koika.Parsing.
+(* Require Import Koika.Parsing. *)
 Require Import Koika.Frontend.
+Require Import Koika.TypedParsing.
 
-Module Import Queue32.
+Module Type QueueParam.
+  Parameter T: type.
+End QueueParam.
+
+Module Queue (QP : QueueParam).
+  Import QP.
+
   Inductive reg_t := empty | data.
   Definition R reg :=
     match reg with
     | empty => bits_t 1
-    | data => bits_t 32
+    | data => T
     end.
 
-  Definition dequeue0: UInternalFunction reg_t empty_ext_fn_t :=
-    {{ fun dequeue0 () : bits_t 32 =>
-         guard(!read0(empty)); write0(empty, Ob~1); read0(data) }}.
+  Definition dequeue0: function R empty_Sigma :=
+    <{ fun dequeue0 () : T =>
+         guard(!read0(empty)); write0(empty, Ob~1); read0(data) }>.
 
-  Definition enqueue0: UInternalFunction reg_t empty_ext_fn_t :=
-    {{ fun enqueue0 (val: bits_t 32) : unit_t =>
-         guard(read0(empty)); write0(empty, Ob~0); write0(data, val) }}.
+  Definition enqueue0: function R empty_Sigma :=
+    <{ fun enqueue0 (val: T) : unit_t =>
+         guard(read0(empty)); write0(empty, Ob~0); write0(data, val) }>.
 
-  Definition dequeue1: UInternalFunction reg_t empty_ext_fn_t :=
-    {{ fun dequeue1 () : bits_t 32 =>
-         guard(!read1(empty)); write1(empty, Ob~1); read1(data) }}.
-End Queue32.
+  Definition dequeue1: function R empty_Sigma :=
+    <{ fun dequeue1 () : T =>
+         guard(!read1(empty)); write1(empty, Ob~1); read1(data) }>.
+
+  Require Import Koika.Hoare.
+  Require Import Koika.Environments.
+
+  (* TODO generalize over sig *)
+  Notation "'{{' P '}}' a '{{' Q '}}'" := (forall REnv, @hoare_triple _ _ _ R empty_Sigma REnv _ _ empty_sigma a P Q) (at level 10, P custom assertion, Q custom ret_assertion, only parsing).
+  From Coq Require Import Utf8.
+
+
+  Theorem simple_hoare_a :
+    ∀ sz n: nat,
+    {{ True }} (<{ a := #n }> : action' R empty_Sigma (sig := [("a", bits_t sz); ("b", bits_t sz)])) {{ Γ[a] = n }}.
+  Proof.
+    hoare.
+  Qed.
+
+  Theorem simple_hoare_b :
+    ∀ sz n m: nat,
+    {{ Γ[a] = n }} (<{ b := #m }> : action' R empty_Sigma (sig := [("a", bits_t sz); ("b", bits_t sz)])) {{ Γ[a] = n /\ Γ[b] = m }}.
+  Proof.
+    hoare. now split.
+  Qed.
+    (* rewrite cassoc_creplace_neq_k. split. assumption. reflexivity. *)
+    (* easy. *)
+  (* Qed. *)
+
+  Theorem simple_hoare :
+    ∀ sz n m: nat,
+    {{ True }} (<{ a := #n; b := #m }> : action' R empty_Sigma (sig := [("a", bits_t sz); ("b", bits_t sz)])) {{ Γ[a] = n /\ Γ[b] = m }}.
+  Proof.
+    intros.
+    eapply hoare_seq.
+    - apply simple_hoare_b.
+    - apply simple_hoare_a.
+  Qed.
+
+  Theorem queue_enc_fail :
+    ∀ n,
+    {{ env[empty] = 0 /\ Γ[a] = n}} (<{ enqueue0(a) }> : action' _ _ (sig := [("a", T)])) {{ False }}.
+  Proof.
+    intros.
+    hoare_step.
+    hoare_step.
+    eapply hoare_args_weaken_pre.
+    hoare_step.
+    hoare_step.
+    hoare_step.
+    hoare_cleanup.
+    hoare_step.
+    hoare.
+    apply (hoare_read (R := R) _ empty).
+    hoare_cleanup. rewrite H.
+    cbn.
+    trivial.
+  Qed.
+
+  Theorem queue_enc_correct :
+    ∀ n: nat,
+    {{ env[empty] = 1 /\ Γ[a] = n }} (<{ enqueue0(a) }> : action' R empty_Sigma (sig := [("a", T)])) {{ env[data] = n /\ env[empty] = 0 }}.
+  Proof.
+    intros.
+    hoare.
+    hoare.
+    apply (hoare_read (R := R) _ empty).
+    hoare_cleanup.
+    rewrite H.
+    hnf.
+    rewrite get_put_eq.
+    let e := eval cbn in (eq_dec data empty) in
+    match e with
+    | right ?Hneq => rewrite (get_put_neq _ _ _ _ _ Hneq)
+    end.
+    rewrite get_put_eq.
+    hoare_cleanup.
+    split. assumption. reflexivity.
+  Qed.
+
+  Theorem queue_deq_correct :
+    ∀ n: nat,
+    {{ env[data] = n /\ env[empty] = 0 }} (<{ dequeue1() }> : action' R empty_Sigma (sig := [("a", T)])) {{ r, r = n }}.
+  Proof.
+    intros.
+    hoare.
+    hoare.
+    apply (hoare_read (R := R) _ data).
+    apply (hoare_read (R := R) _ empty).
+    hoare_cleanup.
+    rewrite H0.
+    hnf.
+    let e := eval cbn in (eq_dec empty data) in
+    match e with
+    | right ?Hneq => rewrite (get_put_neq _ _ _ _ _ Hneq)
+    end.
+    assumption.
+  Qed.
+
+
+  (* Theorem queue_enc_dec : *)
+    (* ∀ sz n: nat,
+    ∀ sig,
+    {{ env[empty] = 1 }} (<{ enqueue0(`Const (@value_of_bits T (Bits.of_nat _ n))`); dequeue1() }> : action' R empty_Sigma (sig := sig)) {{ r, r = n }}.
+  Proof. *)
+  Theorem queue_enc_dec:
+    ∀ n: nat,
+    {{ env[empty] = 1 /\ Γ[a] = n }} (<{ enqueue0(a); dequeue1() }> : action' R empty_Sigma (sig := [("a", T)])) {{ r, r = n }}.
+  Proof.
+    intros.
+    eapply hoare_seq.
+    - apply queue_deq_correct.
+    - apply queue_enc_correct.
+  Qed.
+
+    hoare_step.
+    hoare_step.
+    hoare_step.
+    hoare_step.
+    eapply hoare_args_weaken_pre.
+    hoare_step.
+    hoare_step.
+    hoare_step.
+    hoare_step.
+    hoare_step.
+    unfold enqueue0, action_of_function, int_body, TypedParsing.refine_sig_tau.
+    hoare_step.
+    hoare_step.
+    hoare_step.
+    hoare_step.
+    hoare_step.
+    hoare_step.
+    hoare_step.
+    hoare_step.
+    hoare_step.
+    hoare_step.
+    eapply (hoare_read (R := R) _ empty).
+    with_strategy opaque [ cassoc ] cbn.
+    destruct H.
+    rewrite H.
+    with_strategy opaque [ cassoc ] cbn.
+
+    unfold TypedParsing.refine_sig_tau.
+    hoare_step.
+    hoare_step.
+    hoare_step.
+    eapply (hoare_read (R := R) _ data).
+    hoare_step.
+    hoare_step.
+    hoare_step.
+    hoare_step.
+    hoare_step.
+    hoare_step.
+    hoare_step.
+    eapply (hoare_read (R := R) _ empty).
+    with_strategy opaque [ cassoc ] cbn.
+
+    let e := eval cbn in (eq_dec data empty) in
+    match e with
+    | right ?Hneq => rewrite (get_put_neq _ _ _ _ _ Hneq)
+    end.
+    rewrite get_put_eq.
+    hoare_cleanup.
+    rewrite H0.
+    cbn.
+    unfold ret_assertion_of_assertion.
+    let e := eval cbn in (eq_dec empty data) in
+    match e with
+    | right ?Hneq => rewrite (get_put_neq _ _ _ _ _ Hneq)
+    | left ?Heq => rewrite (get_put_eq _ _ _ _)
+    end.
+    rewrite get_put_eq.
+    reflexivity.
+  Qed.
+End Queue.
+
+Module Type QueueParam'.
+  Parameter T: type. (* type of data which is stored *)
+  Parameter sz: nat. (* number of data items which can be stored *)
+End QueueParam'.
+
+Module Queue' (QP : QueueParam').
+  Import QP.
+
+  Inductive reg_t := empty | data (idx: Vect.index sz).
+  Axiom reg_t_ft : FiniteType reg_t.
+
+  Definition R reg :=
+    match reg with
+    | empty => bits_t 1
+    | data _ => T
+    end.
+
+  Definition dequeue0: function R empty_Sigma :=
+    <{ fun dequeue0 () : T =>
+         guard(!read0(empty)); write0(empty, Ob~1); read0(data) }>.
+
+  Definition enqueue0: function R empty_Sigma :=
+    <{ fun enqueue0 (val: T) : unit_t =>
+         guard(read0(empty)); write0(empty, Ob~0); write0(data, val) }>.
+
+  Definition dequeue1: function R empty_Sigma :=
+    <{ fun dequeue1 () : T =>
+         guard(!read1(empty)); write1(empty, Ob~1); read1(data) }>.
+
+Module QueueParam32 <: QueueParam.
+  Definition T := bits_t 32.
+End QueueParam32.
+Module Import Queue32 := Queue QueueParam32.
 
 Inductive reg_t :=
-| in0: Queue32.reg_t -> reg_t
-| in1: Queue32.reg_t -> reg_t
-| fifo: Queue32.reg_t -> reg_t
-| out: Queue32.reg_t -> reg_t.
+  | in0: Queue32.reg_t -> reg_t
+  | in1: Queue32.reg_t -> reg_t
+  | fifo: Queue32.reg_t -> reg_t
+  | out: Queue32.reg_t -> reg_t.
 
 Inductive rule_name_t := deq0 | deq1 | process.
 
@@ -39,18 +251,18 @@ Definition R (reg: reg_t) : type :=
   | out st => Queue32.R st
   end.
 
-Definition urules (rl: rule_name_t) : uaction reg_t empty_ext_fn_t :=
+Definition rules (rl: rule_name_t) : action R empty_Sigma :=
   match rl with
   | deq0 =>
-    {{ fifo.(enqueue0)(in0.(dequeue0)()) }}
+    <{ fifo.(enqueue0)(in0.(dequeue0)()) }>
   | deq1 =>
-    {{ fifo.(enqueue0)(in1.(dequeue0)()) }}
+    <{ fifo.(enqueue0)(in1.(dequeue0)()) }>
   | process =>
-    {{ out.(enqueue0)(|32`d412| + fifo.(dequeue1)()) }}
+    <{ out.(enqueue0)(|32`d412| + fifo.(dequeue1)()) }>
   end.
 
-Definition rules : rule_name_t -> rule R empty_Sigma :=
-  tc_rules R empty_Sigma urules.
+(* Definition rules : rule_name_t -> rule R empty_Sigma :=
+  tc_rules R empty_Sigma urules. *)
 
 Definition pipeline : scheduler :=
   deq0 |> deq1 |> process |> done.
