examples/method_call.v
@@ -1,28 +1,38 @@
 (*! Calling methods of internal modules !*)
 Require Import Koika.Frontend.
-Require Import Koika.Parsing.
+Require Import Koika.TypedParsing.
 Require Import Koika.Std.
-
 
 Definition ext_fn_t := empty_ext_fn_t.
 
+Module Type DelayParam.
+  Parameter T:type.
+End DelayParam.
+
 (* Definition submodule *)
-Module Delay.
+Module Delay (DP : DelayParam).
+  Import DP.
   Inductive reg_t := buffer.
+  Definition R (r : reg_t) := T.
 
   (* Declaration of a Koika function in a module, called a method *)
-  Definition swap tau: UInternalFunction reg_t ext_fn_t  :=
-    {{
-        fun swap (arg1 : tau) : tau =>
+  Definition swap {Sigma: ext_fn_t -> ExternalSignature}: function R Sigma :=
+    <{
+        fun swap (arg1 : T) : T =>
           write0(buffer, arg1);
           read0(buffer)
-    }}.
+    }>.
 
   Instance FiniteType_reg_t : FiniteType reg_t := _.
 End Delay.
 
+Module DelayParam16 <: DelayParam.
+  Definition T := bits_t 16.
+End DelayParam16.
+Module Delay16 := Delay DelayParam16.
+
 (* Declare state, with submodule instances *)
-Inductive reg_t := rA | rDelay1 (d: Delay.reg_t) | rDelay2 (d: Delay.reg_t).
+Inductive reg_t := rA | rDelay1 (d: Delay16.reg_t) | rDelay2 (d: Delay16.reg_t).
 Inductive rule_name_t := rl.
 
 (* Types of state *)
@@ -42,26 +52,22 @@ Definition r reg : R reg :=
   end.
 
 (* Declaration of a family of Koika function indexed by a coq integer *)
-Definition nor (sz: nat) : UInternalFunction reg_t ext_fn_t :=
-  {{
-      fun nor (arg1 : bits_t sz) (arg2 : bits_t sz) : bits_t sz =>
-        !(arg1 || arg2)
-  }}.
+Definition nor (sz: nat) : function R empty_Sigma := <{
+  fun nor (arg1 : bits_t sz) (arg2 : bits_t sz) : bits_t sz =>
+    !(arg1 || arg2)
+}>.
 
 Definition display :=
   (Display.Printer (ext_fn_t := empty_ext_fn_t) (reg_t := reg_t) (pos_t := pos_t)).
 
-Definition swap16 := Delay.swap (bits_t 16).
-
-Definition _rl : uaction reg_t empty_ext_fn_t :=
-  {{
-      let a := read0(rA) in
-       (* Methods are called as reg.(method)(args...) *)
-      let old_a := rDelay2.(swap16)(a) in
-      (* Parametric functions can be called with {fn params...}(args...) *)
-      write0(rA, {nor 16}(read0(rA), old_a));
-      {display [Display.Str "rA: "; Display.Value (bits_t 16)]}(a)
-  }}.
+Definition _rl : action R empty_Sigma := <{
+  let a := read0(rA) in
+    (* Methods are called as reg.(method)(args...) *)
+  let old_a := rDelay2.(Delay16.swap)(a) in
+  (* Parametric functions can be called with {fn params...}(args...) *)
+  write0(rA, {nor 16}(read0(rA), old_a));
+  {display [Display.Str "rA: "; Display.Value (bits_t 16)]}(a)
+}>.
 
 Definition rules :=
   tc_rules R empty_Sigma
